Disable some low-level parts for now

src/lowparse/LowParse.TestLib.Low.fst
@@ -6,7 +6,7 @@ open FStar.Printf
 open LowParse.Low.Base
 
 module B = LowStar.Buffer
-module I32 = FStar.Int32
+module U32 = FStar.UInt32
 module M = LowStar.Modifies
 
 #reset-options "--using_facts_from '* -LowParse'"
@@ -15,21 +15,21 @@ module M = LowStar.Modifies
 (** The type of a unit test.  It takes an input buffer8, parses it,
     and returns a newly formatted buffer8.  Or it returns None if
     there is a fail to parse. *)
-type testbuffer_t = (input:buffer8) -> (inputlen:I32.t) -> Stack (option (buffer8 * I32.t)) 
-  (requires(fun h -> is_slice h input inputlen ))
+type testbuffer_t = (input: slice) -> ST (option slice) 
+  (requires(fun h -> live_slice h input))
   (ensures(fun h0 y h1 ->
     M.modifies M.loc_none h0 h1 /\ (
     match y with
     | None -> true
-    | Some (r,o) ->
-      B.unused_in r h0 /\
-      is_slice h1 r o
+    | Some out ->
+      B.unused_in out.base h0 /\
+      live_slice h1 out
   )))
 
-assume val load_file_buffer: (filename:string) -> Stack (buffer8 * I32.t)
+assume val load_file_buffer: (filename:string) -> ST slice
   (requires (fun h -> True))
-  (ensures (fun h (y, len) h' ->
-    M.modifies M.loc_none h h' /\ B.unused_in y h /\ is_slice h' y len
+  (ensures (fun h out h' ->
+    M.modifies M.loc_none h h' /\ B.unused_in out.base h /\ live_slice h' out
   ))
 
 (* TODO: implement in LowStar.Buffer *)
@@ -40,7 +40,7 @@ module U32 = FStar.UInt32
 assume
 val beqb: b1:buffer8 -> b2:buffer8
   -> len:U32.t{U32.v len <= B.length b1 /\ U32.v len <= B.length b2}
-  -> ST bool
+  -> Stack bool
     (requires (fun h ->
       B.live h b1 /\
       B.live h b2
@@ -48,20 +48,18 @@ val beqb: b1:buffer8 -> b2:buffer8
     (ensures  (fun h0 z h1 -> h1 == h0 /\
       (z <==> Seq.equal (B.as_seq h0 (B.gsub b1 0ul len)) (B.as_seq h0 (B.gsub b2 0ul len)))))
 
-module Cast = FStar.Int.Cast
-
 (** Test one parser+formatter pair against an in-memory buffer of UInt8.t *)
-let test_buffer (t:testbuffer_t) (testname:string) (input:buffer8) (inputlen:I32.t)
-: Stack unit 
-(requires (fun h -> is_slice h input inputlen))
+let test_buffer (t:testbuffer_t) (testname:string) (input:slice)
+: ST unit 
+(requires (fun h -> live_slice h input))
 (ensures (fun _ _ _ -> true)) =
   push_frame();
   print_string (sprintf "==== Testing buffer %s ====\n" testname);
-  let result = t input inputlen in
+  let result = t input in
   (match result with
-  | Some (formattedresult, offset) -> (
-    if I32.lte offset inputlen then (
-      if beqb input formattedresult (Cast.int32_to_uint32 offset) then
+  | Some output -> (
+    if U32.lte output.len input.len then (
+      if beqb input.base output.base output.len then
         print_string "Formatted data matches original input data\n"
       else (
         print_string "FAIL:  formatted data does not match original input data\n"
@@ -75,8 +73,8 @@ let test_buffer (t:testbuffer_t) (testname:string) (input:buffer8) (inputlen:I32
   pop_frame()
 
 (** Test one parser+formatter pair against a disk file, using buffer *)
-let test_file_buffer (t:testbuffer_t) (filename:string): Stack unit (fun _ -> true) (fun _ _ _ -> true) =
+let test_file_buffer (t:testbuffer_t) (filename:string): ST unit (fun _ -> true) (fun _ _ _ -> true) =
   push_frame();
-  let input, inputlen = load_file_buffer filename in
+  let input = load_file_buffer filename in
   (*test_buffer t filename input inputlen;*)
   pop_frame()
