src/lowparse/LowParse.Low.Array.fst
@@ -1,4 +1,6 @@
 module LowParse.Low.Array
+
+(*
 include LowParse.Spec.Array
 include LowParse.Low.List
 include LowParse.Low.VLData
